feat(Keller/Euclidean): main lemma for Hajos

Experiments/Keller/Euclidean/PeriodicReduction.lean
@@ -1,4 +1,5 @@
 import Experiments.Keller.Euclidean.Basic
+import Experiments.Keller.Euclidean.TilingStructure
 
 namespace Keller.Euclidean
 
@@ -8,14 +9,21 @@ def Tiling.Periodic (T : Tiling d) : Prop :=
 /-- `{0,1}ᵈ` on paper -/
 def PeriodicIndex (d : Nat) := { i : IntPoint d | ∀ j, i j ∈ ({0,1} : Set ℤ) }
 
+theorem PeriodicIndex.mem_iff_real_range : i ∈ PeriodicIndex d ↔ ∀ j, (-1 : ℝ) < i j ∧ i j < (2 : ℝ) := by
+  constructor
+  · intro h j; specialize h j
+    aesop
+  · intro h j
+    suffices -1 < i j ∧ i j < 2 by
+      simp; omega
+    simpa [← Int.cast_lt (R := ℝ)] using h j
+
 /-- if a cube intersects with the origin unit cube `[0,1]ᵈ`,
     then its integer index must be in `{0,1}ᵈ` -/
 theorem PeriodicIndex.of_inter_unitcube_cube_nonempty (h : (UnitCube d ∩ Cube t).Nonempty)
     : Cube.index t ∈ PeriodicIndex d := by
+  rw [PeriodicIndex.mem_iff_real_range]
   intro j
-  suffices -1 < Cube.index t j ∧ Cube.index t j < 2 by
-    simp; omega
-  simp [← Int.cast_lt (R := ℝ)]
   rcases h with ⟨x,x_mem_unit,x_mem_t⟩
   specialize x_mem_unit j
   replace x_mem_t := Cube.close_of_mem_cube x_mem_t (Cube.index_mem _) j
@@ -47,11 +55,11 @@ namespace Hajos
 
 variable (T : Tiling d)
 
-def core := { T.get i | (i ∈ PeriodicIndex d)}
+def core := { t ∈ T.corners | (Cube.index t ∈ PeriodicIndex d)}
 def corners' := {t + (2 • x).toPoint | (t ∈ core T) (x : IntPoint d)}
 
 theorem core_subset_corners : core T ⊆ T.corners := by
-  rintro _ ⟨ti,-,rfl⟩; apply T.get_mem
+  apply Set.sep_subset
 
 theorem core_subset_corners' : core T ⊆ corners' T := by
   rintro t t_mem
@@ -67,18 +75,13 @@ theorem core_covers_unitcube : ∀ x ∈ UnitCube d, ∃! t ∈ core T, x ∈ Cu
   -- this cube corner `t` must be in core because `x ∈ UnitCube d`
   have t_in_core : t ∈ core T := by
     simp [core]
-    obtain i_mem_t :=
-      PeriodicIndex.of_inter_unitcube_cube_nonempty ⟨x,x_mem,x_mem_t⟩
-    use Cube.index t, i_mem_t
-    rw [T.get_index t_corner]
+    use t_corner
+    exact PeriodicIndex.of_inter_unitcube_cube_nonempty ⟨x,x_mem,x_mem_t⟩
 
   use t, ⟨t_in_core,x_mem_t⟩
   -- but we must prove this is unique
   rintro t' ⟨t'_core,x_mem_t'⟩
   refine t_uniq _ ⟨core_subset_corners T t'_core,x_mem_t'⟩
-
-theorem core_can_step_unitcube : ∀ x ∈ UnitCube d, ∀ j : Fin d,
-    x + EuclideanSingle.
 
 /-- BHMN A.3 Fact 1 -/
 theorem corners'_covers_unitcube : ∀ x ∈ UnitCube d, ∃! t ∈ corners' T, x ∈ Cube t := by
@@ -95,17 +98,121 @@ theorem corners'_covers_unitcube : ∀ x ∈ UnitCube d, ∃! t ∈ corners' T, 
     PeriodicIndex.of_inter_unitcube_cube_nonempty ⟨x,x_mem,x_mem_t'⟩
 
   -- and therefore its membership in `corners'` is only possible with offset 0
-  rcases t'_corner with ⟨-,⟨i,i_pidx,rfl⟩,offset,rfl⟩
+  rcases t'_corner with ⟨t',⟨t'_corner,t'_pidx⟩,offset,rfl⟩
   have : offset = 0 := by
-    ext j; specialize this j; specialize i_pidx j
-    rw [Cube.index_add_intpoint, Tiling.index_get] at this
-    simp at i_pidx this ⊢
+    ext j; specialize this j; specialize t'_pidx j
+    rw [Cube.index_add_intpoint] at this
+    simp at t'_pidx this ⊢
     omega
   subst offset; simp [T.index_get] at this ⊢
   -- so `t'` is in `core`
-  have : T.get i.toPoint ∈ core T := ⟨i,this,rfl⟩
+  have : t' ∈ core T := ⟨t'_corner,t'_pidx⟩
   -- and therefore equal to t
   apply t_uniq _ ⟨this,by simpa using x_mem_t'⟩
+
+/-- from the unitcube, we can always step either forward or backward by 1
+    and remain in the core.
+
+    this is heavily modified from BHMN, and is the key lemma
+    used in `corners'_covers` -/
+theorem core_can_step_unitcube : ∀ x ∈ UnitCube d, ∀ j : Fin d,
+    (∃ t ∈ core T, x + .single j 1 ∈ Cube t) ∨
+    (∃ t ∈ core T, x - .single j 1 ∈ Cube t) := by
+  intro x x_mem_unit_cube j
+
+  -- get the core cube containing `x`
+  obtain ⟨t,⟨⟨t_corner,t_pidx⟩,x_mem_t⟩,-⟩ := core_covers_unitcube T x x_mem_unit_cube
+
+  -- we'll need the integral spaced line through `x`
+  have int_spaced_line := ILattice.fromTiling T j |>.inter_line_IntegralSpaced x
+  -- and that `t` intersects the line
+  have t_mem_inter : t ∈ ILattice.inter_line T.corners j x :=
+    ⟨t_corner,x,x_mem_t,Line.start_mem ..⟩
+
+  -- case on whether the index of `t` is 0 or 1 in dimension j
+  cases t_pidx j
+  case inl ti_j =>
+    -- the step forward case
+    left
+
+    -- get the next cube in the line
+    obtain ⟨t',⟨⟨t'_corner,t'_inter_ne⟩,t_j_step⟩,-⟩ := int_spaced_line.exists_unique_next t_mem_inter
+
+    -- `x + eⱼ` is in the `t'` cube
+    have x'_mem_t' : x + .single j 1 ∈ Cube t' := by
+      rw [Point.add_single_eq_update]
+      apply Cube.update_mem_of_inter_line_nonempty _ t'_inter_ne
+      have := (Cube.mem_iff _ _).mp x_mem_t j
+      constructor <;> linarith
+
+    -- and its index is periodic
+    have t'_pidx : Cube.index t' ∈ PeriodicIndex d := by
+      rw [PeriodicIndex.mem_iff_real_range]
+      intro j'
+
+      -- unfold defn of Cube.index and bound the ceil operation
+      simp only [Cube.index] at ti_j ⊢
+      generalize t'i_j' : ⌈t' j'⌉ = t'i
+      simp [Int.ceil_eq_iff] at ti_j t'i_j'
+
+      -- if `j' = j`, we use `next_in_line` to justify the bounds
+      if hj' : j' = j then
+        subst j'
+        constructor <;> linarith
+      -- otherwise, can bound based on `x`
+      else
+        -- since `x ∈ UnitCube d`, we can bound `x j' ∈ [0,1)`
+        specialize x_mem_unit_cube j'
+
+        -- because `x' ∈ Cube t'`, we know `x j' ∈ [t' j', t' j'+1)`
+        replace x'_mem_t' := (Cube.mem_iff _ _).mp x'_mem_t' j'
+
+        simp [hj'] at x'_mem_t'
+        constructor <;> linarith
+
+    use t', ⟨t'_corner,t'_pidx⟩
+
+
+  case inr ti_j =>
+    -- the step backward case. this argument is very very similar to the forward case.
+    right
+
+    -- get the next cube in the line
+    obtain ⟨t',⟨⟨t'_corner,t'_inter_ne⟩,t_j_step⟩,-⟩ := int_spaced_line.exists_unique_prev t_mem_inter
+
+    -- `x - eⱼ` is in the `t'` cube
+    have x'_mem_t' : x - .single j 1 ∈ Cube t' := by
+      rw [sub_eq_add_neg, ← EuclideanSpace.single_neg, Point.add_single_eq_update]
+      apply Cube.update_mem_of_inter_line_nonempty _ t'_inter_ne
+      have := (Cube.mem_iff _ _).mp x_mem_t j
+      constructor <;> linarith
+
+    -- and its index is periodic
+    have t'_pidx : Cube.index t' ∈ PeriodicIndex d := by
+      rw [PeriodicIndex.mem_iff_real_range]
+      intro j'
+
+      -- unfold defn of Cube.index and bound the ceil operation
+      simp only [Cube.index] at ti_j ⊢
+      generalize t'i_j' : ⌈t' j'⌉ = t'i
+      simp [Int.ceil_eq_iff] at ti_j t'i_j'
+
+      -- if `j' = j`, we use `next_in_line` to justify the bounds
+      if hj' : j' = j then
+        subst j'
+        constructor <;> linarith
+      -- otherwise, can bound based on `x`
+      else
+        -- since `x ∈ UnitCube d`, we can bound `x j' ∈ [0,1)`
+        specialize x_mem_unit_cube j'
+
+        -- because `x' ∈ Cube t'`, we know `x j' ∈ [t' j', t' j'+1)`
+        replace x'_mem_t' := (Cube.mem_iff _ _).mp x'_mem_t' j'
+
+        simp [hj'] at x'_mem_t'
+        constructor <;> linarith
+
+    use t', ⟨t'_corner,t'_pidx⟩
 
 theorem split_point (x : Point d) :
       ∃ x_int : IntPoint d, ∃ x_rem ∈ UnitCube d, x = x_int + x_rem := by
@@ -118,8 +225,6 @@ theorem split_point (x : Point d) :
 theorem corners'_covers (p : Point d) : ∃! c, c ∈ corners' T ∧ p ∈ Cube c := by
   obtain ⟨p_int,p_rem,p_rem_mem_unitcube,rfl⟩ := split_point p
 
-  have := core_covers_unitcube T p_rem p_rem_mem_unitcube
-
   -- for every dimension,
   sorry
 
@@ -129,7 +234,7 @@ def T' : Tiling d where
 
 theorem T'_periodic : (T' T).Periodic := by
   simp [T', Tiling.Periodic, corners', core]
-  rintro t i hi x rfl x'
+  rintro t i hi x x'
   use i, hi, x+x'
   ext j; simp [mul_add]; abel
 
